src/Parsers/NonComputational.v
@@ -1,5 +1,5 @@
 (** * Definition of a [comp]-based non-computational CFG parser *)
-Require Import Coq.Lists.List Coq.Program.Program Coq.Program.Wf Coq.Arith.Wf_nat Coq.Arith.Compare_dec Coq.Classes.RelationClasses.
+Require Import Coq.Lists.List Coq.Program.Program Coq.Program.Wf Coq.Arith.Wf_nat Coq.Arith.Compare_dec Coq.Classes.RelationClasses Coq.Strings.String.
 Require Import Parsers.ContextFreeGrammar Parsers.Specification.
 Require Import Common Common.ilist.
 
@@ -74,6 +74,61 @@ Section wf.
       apply well_founded_prod_relation_helper; auto.
     Defined.
   End wf_prod.
+
+  Section wf_sig.
+    Context A B (RA : relation A) (RB : forall a : A, relation (B a)).
+
+    Definition sigT_relation : relation (sigT B)
+      := fun ab a'b' =>
+           RA (projT1 ab) (projT1 a'b') \/ (exists pf : projT1 a'b' = projT1 ab, RB (projT2 ab)
+                                                                                    (eq_rect _ B (projT2 a'b') _ pf)).
+
+    Fixpoint well_founded_sigT_relation_helper
+             a b
+             (wf_A : Acc RA a) (wf_B : forall a, well_founded (@RB a)) {struct wf_A}
+    : Acc sigT_relation (existT _ a b).
+    Proof.
+      refine match wf_A with
+               | Acc_intro fa => (fix wf_B_rec b' (wf_B' : Acc (@RB a) b') : Acc sigT_relation (existT _ a b')
+                                  := Acc_intro
+                                       _
+                                       (fun ab =>
+                                          match ab as ab return sigT_relation ab (existT _ a b') -> Acc sigT_relation ab with
+                                            | existT a'' b'' =>
+                                              fun pf =>
+                                                match pf with
+                                                  | or_introl pf'
+                                                    => @well_founded_sigT_relation_helper
+                                                         _ _
+                                                         (fa _ pf')
+                                                         wf_B
+                                                  | or_intror (ex_intro pfa pfb)
+                                                    => match wf_B' with
+                                                         | Acc_intro fb
+                                                           => _(*eq_rect
+                                                            _
+                                                            (fun a'' => Acc sigT_relation (existT B a'' _(*b''*)))
+                                                            (wf_B_rec _ (fb _ _(*pfb*)))
+                                                            _
+                                                            pfa*)
+                                                       end
+                                                end
+                                          end)
+                                 ) b (wf_B a b)
+             end;
+      simpl in *.
+      destruct pfa; simpl in *.
+      exact (wf_B_rec _ (fb _ pfb)).
+    Defined.
+
+    Definition well_founded_sigT_relation : well_founded RA
+                                            -> (forall a, well_founded (@RB a))
+                                            -> well_founded sigT_relation.
+    Proof.
+      intros wf_A wf_B [a b]; hnf in *.
+      apply well_founded_sigT_relation_helper; auto.
+    Defined.
+  End wf_sig.
 End wf.
 
 Local Open Scope string_like_scope.
@@ -84,32 +139,32 @@ Section recursive_descent_parser.
   depend on the string we're parsing, so we can store proofs in it to
   pass down the parse tree to handle impossible cases.  This will
   require a [Total] lexicographic ordering on strings. *)
-  Context nonterminal_listT
-          (initial_nonterminal_data : nonterminal_listT)
-          (is_valid_nonterminal : nonterminal_listT -> nonterminal CharType -> bool)
-          (remove_nonterminal : nonterminal_listT -> nonterminal CharType -> nonterminal_listT)
-          (nonterminal_listT_R : nonterminal_listT -> nonterminal_listT -> Prop)
-          (remove_nonterminal_dec : forall ls nt, is_valid_nonterminal ls nt = true
-                                                  -> nonterminal_listT_R (remove_nonterminal ls nt) ls)
-          (ntl_wf : well_founded nonterminal_listT_R).
+  Context (nonterminal_listT : String -> Type)
+          (initial_nonterminal_data : forall str, nonterminal_listT str)
+          (is_valid_nonterminal : forall str, nonterminal_listT str -> nonterminal CharType -> bool)
+          (remove_nonterminal : forall str, nonterminal_listT str -> nonterminal CharType -> nonterminal_listT str)
+          (nonterminal_listT_R : forall str, nonterminal_listT str -> nonterminal_listT str -> Prop)
+          (remove_nonterminal_dec : forall str ls nt, is_valid_nonterminal str ls nt = true
+                                                  -> nonterminal_listT_R str (remove_nonterminal str ls nt) ls)
+          (ntl_wf : forall str, well_founded (nonterminal_listT_R str)).
   Section generic.
     Context (T : String -> nonterminal CharType -> Type)
             (T_reverse_lookup : forall str name, T str (Lookup G name) -> T str [ [ NonTerminal _ name ] ]).
     Context (parse_pattern_by_picking
-             : forall max_len
+             : forall str0
                       (parse_pattern_from_split_list'
-                       : forall (strs : list { str : String | Length _ str <= max_len })
+                       : forall (strs : list { str : String | Length _ str < Length _ str0 \/ str = str0 })
                                 (pat : pattern CharType),
                            ilist (fun sp => T (proj1_sig (fst sp)) [ [ snd sp ] ]) (combine strs pat))
                       (str : String)
-                      (pf : Length _ str <= max_len)
+                      (pf : Length _ str < Length _ str0 \/ str = str0)
                       (pat : pattern CharType),
                  T str [ pat ]).
     Context (decide_leaf : forall str ch, T str [ [ Terminal ch ] ]).
     Context (fold_patterns : forall str (pats : list (pattern CharType)),
                                ilist (fun pat => T str [ pat ]) pats
                                -> T str pats).
-    Context (make_abort : forall str nt valid_list, is_valid_nonterminal valid_list nt = false -> T str nt).
+    Context (make_abort : forall str nt valid_list, @is_valid_nonterminal str valid_list nt = false -> T str nt).
 
 
     Section parts.
@@ -125,82 +180,186 @@ Section recursive_descent_parser.
       End item.
 
       Section pattern.
-        Variable max_len : nat.
+        Variable str0 : String.
         Variable parse_nonterminal : forall (str : String)
-                                            (pf : Length _ str <= max_len)
+                                            (pf : Length _ str < Length _ str0 \/ str = str0)
                                             nt, T str nt.
 
         Definition parse_pattern_from_split_list
-                   (strs : list { str : String | Length _ str <= max_len })
+                   (strs : list { str : String | Length _ str < Length _ str0 \/ str = str0 })
                    (pat : pattern CharType)
         : ilist (fun sp => T (proj1_sig (fst sp)) [ [ snd sp ] ]) (combine strs pat)
           := imap_list (fun sp => T (proj1_sig (fst sp)) [ [ snd sp ] ])
-                       (fun sp => parse_item (parse_nonterminal _ (proj2_sig (fst sp))) (snd sp))
+                       (fun sp => parse_item (@parse_nonterminal _ (proj2_sig (fst sp))) (snd sp))
                        (combine strs pat).
 
-        Definition parse_pattern (str : String) (pf : Length _ str <= max_len) (pat : pattern CharType)
+        Definition parse_pattern (str : String) (pf : Length _ str < Length _ str0 \/ str = str0) (pat : pattern CharType)
         : T str [ pat ]
-          := parse_pattern_by_picking parse_pattern_from_split_list str pf pat.
+          := parse_pattern_by_picking parse_pattern_from_split_list pf pat.
       End pattern.
 
       Section nonterminal.
         Section step.
-          Variable max_len : nat.
+          Variable str0 : String.
           Variable parse_nonterminal : forall (str : String)
-                                              (pf : Length _ str <= max_len)
+                                              (pf : Length _ str < Length _ str0 \/ str = str0)
                                               nt, T str nt.
 
-          Definition parse_nonterminal_step (str : String) (pf : Length _ str <= max_len) (nt : nonterminal CharType)
+          Definition parse_nonterminal_step (str : String) (pf : Length _ str < Length _ str0 \/ str = str0) (nt : nonterminal CharType)
           : T str nt
             := fold_patterns (imap_list (fun pat => T str [ pat ])
-                                        (parse_pattern parse_nonterminal str pf)
+                                        (parse_pattern parse_nonterminal pf)
                                         nt).
         End step.
 
         Section wf.
-          Definition parse_nonterminal_or_abort (valid_list : nonterminal_listT) (max_len : nat)
-                     (str : String)
-                     (pf : Length _ str <= max_len)
+          Definition parse_nonterminal_or_abort str0 str (valid_list : forall str, nonterminal_listT str)
+                     (pf : Length _ str < Length _ str0 \/ str = str0)
                      (nt : nonterminal CharType)
           : T str nt.
           Proof.
             revert str pf nt.
-            change max_len with (fst (max_len, valid_list)).
-            generalize (max_len, valid_list); clear max_len valid_list.
-            refine (@Fix (nat * nonterminal_listT) _ (well_founded_prod_relation
-                                                        lt_wf
-                                                        ntl_wf)
+            change str0 with (projT1 (existT nonterminal_listT str0 (valid_list str0))).
+            generalize (existT nonterminal_listT str0 (valid_list str0)); clear str0 valid_list.
+            refine (@Fix (sigT nonterminal_listT) _ (@well_founded_sigT_relation
+                                                       String
+                                                       nonterminal_listT
+                                                       _
+                                                       _
+                                                       (well_founded_ltof _ (Length String))
+                                                       ntl_wf)
                          _ _).
-            intros [max_len valid_list] parse_nonterminal str pf nt.
-            apply le_lt_eq_dec in pf; simpl in *.
-            destruct pf as [pf|pf].
+            intros [str0 valid_list] parse_nonterminal str pf nt; simpl in *.
+            destruct (lt_dec (Length _ str) (Length _ str0)) as [pf'|pf'];
+              [ | assert (str = str0) by intuition; subst ].
             { (** [str] got smaller, so we reset the valid nonterminals *)
-              destruct max_len as [|max_len]; [ solve [ destruct (Lt.lt_n_0 _ pf) ] | ].
               specialize (parse_nonterminal
-                            (max_len, initial_nonterminal_data)
-                            (or_introl (Lt.lt_n_Sn _))).
-              apply le_S_n in pf.
-              exact (parse_nonterminal_step parse_nonterminal str pf nt). }
+                            (existT _ str (initial_nonterminal_data str))
+                            (or_introl pf')); simpl in *.
+              exact (parse_nonterminal_step parse_nonterminal (or_intror eq_refl) nt). }
             { (** [str] didn't get smaller, so we cache the fact that we've hit this nonterminal already *)
               case_eq (is_valid_nonterminal valid_list nt).
               { (** It was valid, so we can remove it *)
                 intro H.
-                specialize (parse_nonterminal
-                              (max_len, remove_nonterminal valid_list nt)
-                              (or_intror (conj (reflexivity _) (remove_nonterminal_dec H)))).
-                apply NPeano.Nat.eq_le_incl in pf.
-                exact (parse_nonterminal_step parse_nonterminal str pf nt). }
+                specialize (fun pf' => parse_nonterminal
+                              (existT _ str0 (remove_nonterminal valid_list nt))
+                              (or_intror (ex_intro _ eq_refl pf'))); simpl in *.
+                specialize (parse_nonterminal (remove_nonterminal_dec H)).
+                exact (parse_nonterminal_step parse_nonterminal (or_intror eq_refl) nt). }
               { (** oops, we already saw this nonterminal in the past.  ABORT! *)
                 apply make_abort. } }
           Defined.
 
           Definition parse_nonterminal str nt : T str nt
-            := @parse_nonterminal_or_abort initial_nonterminal_data (Length _ str) str
-                                           (NPeano.Nat.eq_le_incl _ _ (reflexivity _)) nt.
+            := @parse_nonterminal_or_abort str str initial_nonterminal_data
+                                           (or_intror eq_refl) nt.
         End wf.
       End nonterminal.
     End parts.
   End generic.
+
+  Section parse_tree_no_split.
+    Local Hint Constructors parse_of parse_of_pattern parse_of_item : parse_tree.
+    Local Hint Resolve ParseHead ParsePatternSingleton : parse_tree.
+    Local Hint Extern 1 => apply ParseHead : parse_tree.
+    Local Hint Extern 0 (option (parse_of _ _ _ [])) => exact None : parse_tree.
+
+    Definition parse_tree_no_split_for : forall str nt, option (parse_of String G str nt).
+    Proof with auto with parse_tree nocore.
+      apply (@parse_nonterminal (fun str nt => option (parse_of _ G str nt))).
+      { intros str name [p|]; [ apply Some | exact None ]... }
+      { intros.
+        specialize (parse_pattern_from_split_list' ((exist _ str pf)::nil) pat); simpl in *.
+        destruct pat as [|pat0 [|pat1 pats] ]; simpl in *.
+        { case_eq (str =s Empty _); intro H; [ apply Some | exact None ]...
+          apply bool_eq_correct in H; subst... }
+        { destruct (ilist_hd parse_pattern_from_split_list') as [tree|]; simpl in *; [ apply Some | exact None ]... }
+        { (** we don't handle the case where we need to split the string *)
+          exact None. } }
+      { (** decide_leaf *)
+        intros str ch.
+        case_eq (str =s [[ch]]); intro H; [ apply bool_eq_correct in H; apply Some | exact None ].
+        subst... }
+      { (** fold_patterns *)
+        intros str pats parses; induction parses; simpl in *...
+        repeat match goal with H : option _ |- _ => destruct H end;
+          try solve [ apply Some; auto with parse_tree nocore
+                    | apply Some;
+                      repeat match goal with
+                               | _ => progress auto with parse_tree nocore
+                               | [ H : parse_of _ _ _ _ |- _ ] => inversion H; clear H; subst
+                             end
+                    | match goal with
+                        | [ H : parse_of _ _ _ _ |- _ ] => fail 1
+                        | _ => idtac
+                      end;
+                      exact None ]. }
+      { (** make_abort *)
+        intros; exact None. }
+    Defined.
+  End parse_tree_no_split.
+End recursive_descent_parser.
+
+Section recursive_descent_parser_list.
+  Context {CharType} {String : string_like CharType} {G : grammar CharType}.
+  Variable (CharType_eq_dec : forall x y : CharType, {x = y} + {x <> y}).
+  Definition rdp_list_nonterminal_listT : String -> Type := fun _ => list (nonterminal CharType).
+  Definition rdp_list_is_valid_nonterminal : forall str, rdp_list_nonterminal_listT str -> nonterminal CharType -> bool
+    := fun str ls nt => if in_dec (nonterminal_dec CharType_eq_dec) nt ls then true else false.
+  Definition rdp_list_remove_nonterminal : forall str, rdp_list_nonterminal_listT str -> nonterminal CharType -> rdp_list_nonterminal_listT str
+    := fun str ls nt =>
+         filter (fun x => if nonterminal_dec CharType_eq_dec nt x then false else true) ls.
+  Definition rdp_list_nonterminal_listT_R : forall str, rdp_list_nonterminal_listT str -> rdp_list_nonterminal_listT str -> Prop
+    := fun _ => ltof _ (@List.length _).
+  Lemma filter_list_dec {T} f (ls : list T) : List.length (filter f ls) <= List.length ls.
+  Proof.
+    induction ls; trivial; simpl in *.
+    repeat match goal with
+             | [ |- context[if ?a then _ else _] ] => destruct a; simpl in *
+             | [ |- S _ <= S _ ] => solve [ apply Le.le_n_S; auto ]
+             | [ |- _ <= S _ ] => solve [ apply le_S; auto ]
+           end.
+  Defined.
+  Lemma rdp_list_remove_nonterminal_dec : forall str ls nt, @rdp_list_is_valid_nonterminal str ls nt = true
+                                                            -> @rdp_list_nonterminal_listT_R str (@rdp_list_remove_nonterminal str ls nt) ls.
+  Proof.
+    intros.
+    unfold rdp_list_is_valid_nonterminal, rdp_list_nonterminal_listT_R, rdp_list_remove_nonterminal, ltof in *.
+    destruct (in_dec (nonterminal_dec CharType_eq_dec) nt ls); [ | discriminate ].
+    match goal with
+      | [ H : In ?nt ?ls |- context[filter ?f ?ls] ]
+        => assert (~In nt (filter f ls))
+    end.
+    { intro H'.
+      apply filter_In in H'.
+      destruct H' as [? H'].
+      destruct (nonterminal_dec CharType_eq_dec nt nt); congruence. }
+    { match goal with
+        | [ |- context[filter ?f ?ls] ] => generalize dependent f; intros
+      end.
+      induction ls; simpl in *; try congruence.
+      repeat match goal with
+               | [ |- context[if ?x then _ else _] ] => destruct x; simpl in *
+               | [ H : _ \/ _ |- _ ] => destruct H
+               | _ => progress subst
+               | [ H : ~(_ \/ _) |- _ ] => apply Decidable.not_or in H
+               | [ H : _ /\ _ |- _ ] => destruct H
+               | [ H : ?x <> ?x |- _ ] => exfalso; apply (H eq_refl)
+               | _ => apply Lt.lt_n_S
+               | _ => apply Le.le_n_S
+               | _ => apply filter_list_dec
+               | [ H : _ -> _ -> ?G |- ?G ] => apply H; auto
+             end. }
+  Defined.
+  Lemma rdp_list_ntl_wf : forall str, well_founded (@rdp_list_nonterminal_listT_R str).
+  Proof.
+    unfold rdp_list_nonterminal_listT_R.
+    intro.
+    apply well_founded_ltof.
+  Defined.
+End recursive_descent_parser_list.
+
+(*
 
   Section parse_tree.
     Context (make_splits : forall (str : String) (pat : pattern CharType),
@@ -281,3 +440,32 @@ Print Universes.
 End recursive_descent_parser.
 
 Section
+*)
+
+
+Module example_parse_empty_grammar.
+  Definition make_parse_of : forall str nt, option (parse_of string_stringlike (trivial_grammar _) str nt).
+  Proof.
+    eapply parse_tree_no_split_for
+    with (nonterminal_listT := rdp_list_nonterminal_listT)
+           (is_valid_nonterminal := rdp_list_is_valid_nonterminal Ascii.ascii_dec)
+           (remove_nonterminal := rdp_list_remove_nonterminal Ascii.ascii_dec)
+           (nonterminal_listT_R := rdp_list_nonterminal_listT_R).
+    { intros; exact [Lookup (trivial_grammar _) ""%string]. }
+    { apply rdp_list_remove_nonterminal_dec. }
+    { apply rdp_list_ntl_wf. }
+  Defined.
+
+  Definition parse : forall str : string, option (parse_of string_stringlike (trivial_grammar _) str (trivial_grammar _))
+    := fun str => make_parse_of str _.
+
+  Eval hnf in if (parse "") then true else false.
+  Eval hnf in if (parse "a") then true else false.
+
+  Goal True.
+    pose (parse "") as X.
+    hnf in X; simpl in X.
+    pose (parse "a") as Y.
+    hnf in Y; simpl in Y.
+  Abort.
+End example_parse_empty_grammar.
